
$$A \cdot \vec{v} = 
\begin{bmatrix}
a & b \\
c & d \\
\end{bmatrix} \cdot
\begin{bmatrix}
x \\
y \\
\end{bmatrix} =
\begin{bmatrix}
ax + by \\
cx + dy \\
\end{bmatrix}
\\
B \cdot (A \cdot \vec{v}) = 
\begin{bmatrix}
e & f \\
g & h \\
\end{bmatrix} \cdot
\begin{bmatrix}
ax + by \\
cx + by \\
\end{bmatrix} =
\begin{bmatrix}
e(ax + by) + f(cx + dy) \\
g(ax + by) + h(cx + dy) \\
\end{bmatrix}
$$

$$B \cdot A =
\begin{bmatrix}
e & f \\
g & h \\
\end{bmatrix} \cdot
\begin{bmatrix}
a & b \\
c & d \\
\end{bmatrix} =
\begin{bmatrix}
ae + cf & be + df \\
ag + ch & bg + dh \\
\end{bmatrix}
\\
(B \cdot A) \cdot \vec{v} = 
\begin{bmatrix}
x(ae + cf) + y(be + df) \\
x(ag + ch) + y(bg + dh) \\
\end{bmatrix}
$$
